riscV/CSE2depsproof.v
@@ -1,0 +1,129 @@
+Require Import Coqlib Maps Errors Integers Floats Lattice Kildall.
+Require Import AST Linking.
+Require Import Memory Registers Op RTL Maps.
+
+Require Import Globalenvs Values.
+Require Import Linking Values Memory Globalenvs Events Smallstep.
+Require Import Registers Op RTL.
+Require Import CSE2 CSE2deps.
+Require Import Lia.
+
+Lemma ptrofs_size :
+  Ptrofs.wordsize = (if Archi.ptr64 then 64 else 32)%nat.
+Proof.
+  unfold Ptrofs.wordsize.
+  unfold Wordsize_Ptrofs.wordsize.
+  trivial.
+Qed.
+
+Lemma ptrofs_modulus :
+  Ptrofs.modulus = if Archi.ptr64 then 18446744073709551616 else 4294967296.
+Proof.
+  unfold Ptrofs.modulus.
+  rewrite ptrofs_size.
+  destruct Archi.ptr64; reflexivity.
+Qed.
+
+Section SOUNDNESS.
+  Variable F V : Type.
+  Variable genv: Genv.t F V.
+  Variable sp : val.
+
+Section MEMORY_WRITE.
+  Variable m m2 : mem.
+  Variable chunkw chunkr : memory_chunk.
+  Variable base : val.
+  
+  Variable addrw addrr valw valr : val.
+  Hypothesis STORE : Mem.storev chunkw m addrw valw = Some m2.
+  Hypothesis READ : Mem.loadv chunkr m addrr = Some valr.
+
+  Section INDEXED_AWAY.
+  Variable ofsw ofsr : ptrofs.
+  Hypothesis ADDRW : eval_addressing genv sp
+                       (Aindexed ofsw) (base :: nil) = Some addrw. 
+  Hypothesis ADDRR : eval_addressing genv sp
+                       (Aindexed ofsr) (base :: nil) = Some addrr.
+
+  Lemma load_store_away1 :
+    forall RANGEW : 0 <= Ptrofs.unsigned ofsw <= Ptrofs.modulus - largest_size_chunk,
+    forall RANGER : 0 <= Ptrofs.unsigned ofsr <= Ptrofs.modulus - largest_size_chunk,
+    forall SWAPPABLE :    Ptrofs.unsigned ofsw + size_chunk chunkw <= Ptrofs.unsigned ofsr
+                       \/ Ptrofs.unsigned ofsr + size_chunk chunkr <= Ptrofs.unsigned ofsw,
+    Mem.loadv chunkr m2 addrr = Some valr.
+  Proof.
+    intros.
+    
+    pose proof (max_size_chunk chunkr) as size_chunkr_bounded.
+    pose proof (max_size_chunk chunkw) as size_chunkw_bounded.
+    unfold largest_size_chunk in *.
+
+    rewrite ptrofs_modulus in *.
+    simpl in *.
+    inv ADDRR.
+    inv ADDRW.
+    rewrite <- READ.
+    destruct base; try discriminate.
+    eapply Mem.load_store_other with (chunk := chunkw) (v := valw) (b := b).
+    exact STORE.
+    right.
+
+    all: try (destruct (Ptrofs.unsigned_add_either i ofsr) as [OFSR | OFSR];
+              rewrite OFSR).
+    all: try (destruct (Ptrofs.unsigned_add_either i ofsw) as [OFSW | OFSW];
+              rewrite OFSW).
+    all: try rewrite ptrofs_modulus in *.
+    all: destruct Archi.ptr64.
+
+    all: intuition lia.
+  Qed.
+  
+  Theorem load_store_away :
+    can_swap_accesses_ofs (Ptrofs.unsigned ofsr) chunkr (Ptrofs.unsigned ofsw) chunkw = true ->
+    Mem.loadv chunkr m2 addrr = Some valr.
+  Proof.
+    intro SWAP.
+    unfold can_swap_accesses_ofs in SWAP.
+    repeat rewrite andb_true_iff in SWAP.
+    repeat rewrite orb_true_iff in SWAP.
+    repeat rewrite Z.leb_le in SWAP.
+    apply load_store_away1.
+    all: tauto.
+  Qed.
+  End INDEXED_AWAY.
+End MEMORY_WRITE.
+End SOUNDNESS.
+
+
+Section SOUNDNESS.
+  Variable F V : Type.
+  Variable genv: Genv.t F V.
+  Variable sp : val.
+
+Lemma may_overlap_sound:
+  forall m m' : mem,
+  forall chunk addr args chunk' addr' args' v a a' vl rs,
+    (eval_addressing genv sp addr (rs ## args)) = Some a ->
+    (eval_addressing genv sp addr' (rs ## args')) = Some a' ->
+    (may_overlap chunk addr args chunk' addr' args') = false ->
+    (Mem.storev chunk m a v) = Some m' ->
+    (Mem.loadv chunk' m  a') = Some vl ->
+    (Mem.loadv chunk' m' a') = Some vl.
+Proof.
+  intros until rs.
+  intros ADDR ADDR' OVERLAP STORE LOAD.
+  destruct addr; destruct addr'; try discriminate.
+  { (* Aindexed / Aindexed *)
+  destruct args as [ | base [ | ]]. 1,3: discriminate.
+  destruct args' as [ | base' [ | ]]. 1,3: discriminate.
+  simpl in OVERLAP.
+  destruct (peq base base'). 2: discriminate.
+  subst base'.
+  destruct (can_swap_accesses_ofs (Ptrofs.unsigned i0) chunk' (Ptrofs.unsigned i) chunk) eqn:SWAP.
+  2: discriminate.
+  simpl in *.
+  eapply load_store_away with (F:=F) (V:=V) (genv:=genv) (sp:=sp); eassumption.
+  }
+Qed.
+
+End SOUNDNESS.
